lakefile.lean
@@ -5,7 +5,7 @@ package «verity-benchmark» where
   version := v!"0.1.0"
 
 require verity from git
-  "https://github.com/lfglabs-dev/verity.git"@"f28f1ba4d7741f2f0794c0571cd181e480d5a5fd"
+  "https://github.com/lfglabs-dev/verity.git"@"b2f2ee402fd56b59e19df39752f7da039f3df4eb"
 
 @[default_target]
 lean_lib «Benchmark» where
